
$$
If\ y\ =\ f(x)\ be\ a\ general\ function\ of\ x,\ then\ its\ differential\ coefficient\ y_1\ =\ \frac{dy}{dx}\ =\ f^`(x)\ is
$$
$$
called\ the\ first\ derivative\ of\ f(x).\ The\ differential\ coefficient\ of\ f^`(x)\ is\ called\ the\ 2nd
$$
$$
derivative\ of\ f(x)\ and\ it\ is\ denoted\ by\ f^{``}(x).\ Similarly,\ the\ differential\ coefficient\ of\ f^{``}(x)\ is
$$
$$
called\ the\ 3rd\ derivative\ of\ f(x)\ and\ it\ is\ denoted\ by\ f^{```}(x)\ and\ so\ on.\ If\ f(x)\ is\ differentiated\ n
$$
$$
times\ with\ respect\ to\ x\ then\ it\ is\ called\ the\ nth\ derivative\ of\ f(x)\ and\ it\ is\ denoted\ by\ f^n(x).\ So\ the
$$
$$
successive\ derivatives\ of\ y\ =\ f(x)\ are\ denoted\ by\ f^`(x),\ f^{``}(x),\ f^{```}(x),\ ... \ ...,\ f^n(x),\ ...\ ...\ ...
$$



# Leibnitz's Theorem

Statement: If *u* and *v* are two functions of *x*, then the nth derivative of their product is

$$
(uv)_n\ =\ u_nv\ +\ n_{C_1}u_{n - 1}v\ +\ n_{C_2}u_{n - 2}v_2\ +\ ...\ ...\ +\ n_{C_r}u_{n - r}v_r \ +\ uv_n
$$
Where the suffixes in *u* and *v* denote the order of derivations of *u* and *v* with respect to *x*.


# Proof of Leibnitz's Theorem


$$
Let,\ y\ =\ uv
$$
$$
y_1\ =\ u_1v\ +\ uv_1
$$
$$
y_2\ =\ u_2v\ +\ u_1v_1\ +\ u_1v_1\ +\ uv_2
$$
$$
=\ u_2v\ +\ 2_{C_1}u_{2-1}v_1\ +\ uv_2
$$
Similarly,
$$
y_3\ =\ u_3v\ +\ u_2v_1\ +\ 2u_2v_1\ +\ 2u_1v_2\ +\ u_1v_2\ +\ uv_3
$$
$$
=\ u_3v\ +\ 3_{C_1}u_{3-1}v_1\ +\ 3_{C_2}u_{3-2}v_2\ +\ uv_3
$$
$$
...\ ...\ ...
$$
$$
y_n\ =\ u_nv\ +\ n_{C_1}u_{n - 1}v\ +\ n_{C_2}u_{n - 2}v_2\ +\ ...\ ...\ +\ n_{C_r}u_{n - r}v_r \ +\ uv_n
$$
