

# Tangent

**The tangent at any point $P$ to a given curve is defined as the limiting position of the secant $PQ$ as the point $Q$ approaches $P$ along the curve.**

$(i)$ Let the equation of the curve be $y = f(x)$ and the given point $P$ on the curve is $(x, y)$ and any other neighboring point $Q$ on the curve is $(x + \Delta x, y + \Delta y)$.

The equation of the secant $PQ$ is 
$$
\frac{Y - y}{X - x} = \frac{y + \Delta y - y}{x + \Delta x - x}
$$
$$
or, Y - y = \frac {\Delta x}{\Delta y}(X - x)
$$
So, the equation of the tangent at P is
$$
or, Y - y = \lim_{\Delta x \to 0} \frac{\Delta y}{\Delta x}(X - x)
$$
$$
or, Y - y = \frac{dy}{dx}(X - x)\ .....(i)
$$

$(ii)$ When the equation of the curve is $f(x, y)$ = 0 then the equation of the tangent to the curve at $(x, y)$ is $(X - x)f_x + (Y - y)f_y = 0\ .....(ii)$

$(iii)$ When the equation of the curve is $x = \phi(t)$, $y = \psi(t)$ then the equation of the tangent to the curve at $'t'$ is $\psi'(t)X - \phi'(t)Y = \phi(t)\psi'(t) - \psi(t)\phi'(t)$       




# Normal

**The normal at any point P to a given curve is the straight line through that point drawn perpendicular to the tangent at that point P**

$(i)$ The normal of the curve $y = f(x)$ at $(x, y)$ is
$$
\frac{dy}{dx}(Y - y) + (X - x) = 0
$$
$(ii)$ When the equation of the curve is $f(x, y) = 0$ then the equation of the normal at $(x, y)$ is $\frac{X - x}{f_x} = \frac{Y - y}{f_y}$

$(iii)$ When the equation of the curve is $x = \phi(t)$, $y = \psi(t)$ then the equation of the normal at $'t'$ is $\phi'(t)X + \psi'(t)Y = \phi(t)\phi'(t) + \psi(t)\psi'(t)\ ......(iii)$
